cfrontend/BeePL_compiler_proofs.v
@@ -327,15 +327,15 @@ Qed. *)
 Admitted.
 
 (* Relation between BeePL vmap and Csyntax local env *)
-Record match_env (vm : BeePL.vmap) (cvm : env) : Prop :=
+Record match_env (venv : renv) (vm : BeePL.vmap) (cvm : env) : Prop :=
 mk_match_env {
  local_match: forall id b t ct,
               vm!id = Some (b, t) ->
               transBeePL_type t = ct ->
-              cvm!id = Some (b, ct);
+              cvm!(resolve venv id) = Some (b, ct);
  global_match: forall id,
                vm!id = None ->
-               cvm!id = None }.
+               cvm!(resolve venv id) = None }.
 
 End specifications.
 
@@ -353,8 +353,8 @@ Admitted.
 
 (* Medium *)
 (* Preservation of symbols *) 
-Lemma symbols_preserved : forall bge cge (id : ident), 
-Genv.find_symbol (Csem.genv_genv cge) id = Genv.find_symbol (BeePL.genv_genv bge) id.
+Lemma symbols_preserved : forall venv bge cge (id : ident), 
+Genv.find_symbol (Csem.genv_genv cge) (resolve venv id) = Genv.find_symbol (BeePL.genv_genv bge) id.
 Proof.
 Admitted.
 
@@ -365,22 +365,22 @@ Proof.
 Admitted.
 
 (* Equivalence between vmaps benv and cenv *)
-Lemma equiv_global_benv_cenv : forall benv cenv vi, 
-match_env benv cenv ->
+Lemma equiv_global_benv_cenv : forall venv benv cenv vi, 
+match_env venv benv cenv ->
 benv ! vi = None ->
-cenv ! vi = None.
+cenv ! (resolve venv vi) = None.
 Proof.
-move=> benv cenv vi h hm. case hb: (cenv ! vi)=> [ [l t] | ] //=.
+move=> venv benv cenv vi h hm. case hb: (cenv ! (resolve venv vi))=> [ [l t] | ] //=.
 case h=> //= h' h''. move: (h'' vi hm)=> hc. by rewrite hc in hb.
 Qed.
 
-Lemma equiv_local_benv_cenv : forall benv cenv vi l t ct, 
-match_env benv cenv ->
+Lemma equiv_local_benv_cenv : forall venv benv cenv vi l t ct, 
+match_env venv benv cenv ->
 transBeePL_type t = ct ->
 benv ! vi = Some (l, t) ->
-cenv ! vi = Some (l, ct).
+cenv ! (resolve venv vi) = Some (l, ct).
 Proof.
-move=> benv cenv vi l t ct h ht hm. 
+move=> venv benv cenv vi l t ct h ht hm. 
 case h=> //= h' h''. by move: (h' vi l t ct hm ht). 
 Qed.
 
@@ -507,7 +507,7 @@ transBeePL_expr_expr e venv fctx bctx g = Res (ce, f, b) g' i' ->
 match e with
 | Val v t => ce = Eval (trans_bvalue_cvalue v) (transBeePL_type t)
              /\ f = fctx /\ b = bctx
-| Var x t => ce = Csyntax.Evar x (transBeePL_type t)
+| Var x t => ce = Csyntax.Evar (resolve venv x) (transBeePL_type t)
              /\ f = fctx /\ b = bctx
 | Const (ConsInt i) t => ce = Eval (Values.Vint i) (transBeePL_type t)
                          /\ f = fctx /\ b = bctx 
@@ -572,17 +572,21 @@ match e with
 | Prim (Cast t) es t' => exists ces g1 i1,
                          transBeePL_expr_exprs transBeePL_expr_expr es venv fctx bctx g = Res (ces, f, b) g1 i1 /\
                          ce = Csyntax.Ecast (hd default_expr (exprlist_list_expr ces)) (transBeePL_type t)
-| Bind x t e1 e2 t' => exists ce1 fctx1 bctx1 g1 i1 ce2 g2 i2,
-                       transBeePL_expr_expr e1 venv fctx bctx g = Res (ce1, fctx1, bctx1) g1 i1 /\
-                       transBeePL_expr_expr e2 venv fctx1 bctx1 g1 = Res (ce2, f, b) g2 i2 /\
-                       if (x =? Ctypesdefs.ident_of_string "_")%positive 
-                       then ce = Ecomma ce1 ce2 (transBeePL_type t')
-                       else ce = Ecomma (Eassign (Csyntax.Evar x (transBeePL_type t)) ce1 (transBeePL_type t)) ce2 (transBeePL_type t')
+| Bind x t e1 e2 t' => if (x =? Ctypesdefs.ident_of_string "_")%positive 
+                       then exists ce1 fctx1 bctx1 g1 i1 ce2 g2 i2,
+                            transBeePL_expr_expr e1 venv fctx bctx g = Res (ce1, fctx1, bctx1) g1 i1 /\
+                            transBeePL_expr_expr e2 venv fctx1 bctx1 g1 = Res (ce2, f, b) g2 i2 /\ 
+                            ce = Ecomma ce1 ce2 (transBeePL_type t')
+                       else exists ce1 fctx1 bctx1 g1 i1 ce2 cx tag g2 i2 g3 i3,
+                            transBeePL_expr_expr e1 venv fctx bctx g = Res (ce1, fctx1, bctx1) g1 i1 /\ 
+                            fresh_ident (List.map unzip_ident fctx1) max_fresh g1 = Res (cx, tag) g2 i2 /\
+                            transBeePL_expr_expr e2 (extend venv x cx) ((cx, t, tag) :: fctx1) bctx1 g2 = Res (ce2, f, b) g3 i3 /\
+                            ce = Ecomma (Eassign (Csyntax.Evar cx (transBeePL_type t)) ce1 (transBeePL_type t)) ce2 (transBeePL_type t')
 | Cond e1 e2 e3 t => exists ce1 fctx1 bctx1 g1 i1 ce2 fctx2 bctx2 g2 i2 ce3 g3 i3,
                      transBeePL_expr_expr e1 venv fctx bctx g = Res (ce1, fctx1, bctx1) g1 i1 /\
                      transBeePL_expr_expr e2 venv fctx1 bctx1 g1 = Res (ce2, fctx2, bctx2) g2 i2 /\
                      transBeePL_expr_expr e3 venv fctx2 bctx2 g2 = Res (ce3, f, b) g3 i3 /\
-                     eq_type t (typeof_expr e2) && eq_type t (typeof_expr e3) /\
+                     (*eq_type t (typeof_expr e2) && eq_type t (typeof_expr e3) /\*)
                      ce = Econdition ce1 ce2 ce3 (transBeePL_type t)
 | _ => True
 end) /\
@@ -596,10 +600,10 @@ end) /\
               ces = Econs ce ce' /\ f = f'' /\ b = b''
 end).
 Proof.
-(*split. 
+split. 
 + move=> e venv fctx bctx ce f b g g' i'. elim: e.
   + move=> v t /=. by move=> [] h1 h2 h3 h4; subst. 
-  + by move=> x t /= [] h1 h2 h3 h4; subst.
+  + by move=> x t /= [] h1 h2 h3 h4; subst;split=> //=.
   + move=> c t /=. case: c=> //=.
     + move=> bo []. case: ifP=> //=.
       + move=> heq [] h1 h2 h3 h4; subst. by case: bo heq=> //=.
@@ -627,21 +631,21 @@ Proof.
       by case: res h hes hfr=> [[a b] c]; subst; case: fr=> [f1 f2];split=> //=.
    (* deref *)
    + move=> es t h. inversion h. rewrite /SimplExpr.bind2 /SimplExpr.bind in H0.
-     case hes: (transBeePL_expr_exprs transBeePL_expr_expr es fctx bctx g) H0=> [errs | ces g1 i1] //=.
+     case hes: (transBeePL_expr_exprs transBeePL_expr_expr es venv fctx bctx g) H0=> [errs | ces g1 i1] //=.
      move=> [] h1 h2 h3 h4; subst. exists ces.1.1, g', i1. by case: (ces)=> [[a b] c]; split=> //=.
    (* massgn *)       
    + move=> es t h. inversion h. rewrite /SimplExpr.bind2 /SimplExpr.bind in H0.
-     case hes: (transBeePL_expr_exprs transBeePL_expr_expr es fctx bctx g) H0=> [errs | ces g1 i1] //=.
+     case hes: (transBeePL_expr_exprs transBeePL_expr_expr es venv fctx bctx g) H0=> [errs | ces g1 i1] //=.
      move=> [] h1 h2 h3 h4; subst. exists ces.1.1, g', i1. split=> //=.
      by case: (ces)=> [[a b] c] //=.
    (* uop *)
    + move=> uop es t h. inversion h. rewrite /SimplExpr.bind2 /SimplExpr.bind in H0.
-     case hes: (transBeePL_expr_exprs transBeePL_expr_expr es fctx bctx g) H0=> [errs | ces g1 i1] //=.
+     case hes: (transBeePL_expr_exprs transBeePL_expr_expr es venv fctx bctx g) H0=> [errs | ces g1 i1] //=.
      move=> [] h1 h2 h3 h4; subst. exists ces.1.1, g', i1. split=> //=.
      by case: (ces)=> [[a b] c] //=.
    (* bop *)
    + move=> bop es t h. inversion h. rewrite /SimplExpr.bind2 /SimplExpr.bind in H0.
-     case hes: (transBeePL_expr_exprs transBeePL_expr_expr es fctx bctx g) H0=> [errs | ces g1 i1] //=.
+     case hes: (transBeePL_expr_exprs transBeePL_expr_expr es venv fctx bctx g) H0=> [errs | ces g1 i1] //=.
      case: bop h=> //=.
      + move=> h [] h1 h2 h3 h4; subst. 
        exists ces.1.1, g', i1; split=> //=. by case: (ces) => [[a b] c].
@@ -690,35 +694,36 @@ Proof.
   (* cast *)
   move=> t es t' hte. inversion hte; subst.
   rewrite /SimplExpr.bind2 /SimplExpr.bind in H0.
-  case hes: (transBeePL_expr_exprs transBeePL_expr_expr es fctx bctx g) H0=> [errs | ces g1 i1] //=.
+  case hes: (transBeePL_expr_exprs transBeePL_expr_expr es venv fctx bctx g) H0=> [errs | ces g1 i1] //=.
   move=> [] h1 h2 h3 h4; subst. exists ces.1.1, g', i1; split=> //=. by case: (ces)=> [[a b] c].
 (* Bind *)
 + move=> x t e1 hte1 e2 hte2 t' hte. inversion hte; subst. 
   case hp : (x =? 126%AC)%positive H0=> //=.
   + rewrite hp /=. rewrite /SimplExpr.bind2 /SimplExpr.bind /=.
-    case he1: (transBeePL_expr_expr e1 fctx bctx g)=> [err1 | ce1 g1 i1] //=.
-    case he2 : (transBeePL_expr_expr e2 ce1.1.2 ce1.2 g1)=> [err2 | ce2 g2 i2] //=.
+    case he1: (transBeePL_expr_expr e1 venv fctx bctx g)=> [err1 | ce1 g1 i1] //=.
+    case he2 : (transBeePL_expr_expr e2 venv ce1.1.2 ce1.2 g1)=> [err2 | ce2 g2 i2] //=.
     move=> [] h1 h2 h3 h4; subst. exists ce1.1.1, ce1.1.2, ce1.2, g1, i1, ce2.1.1, g', i2.
     split=> //=. + by case: (ce1) => [[a b] c].
     split=> //=. by case: (ce2) he2=> [[a b] c].
   rewrite hp /=. rewrite /SimplExpr.bind2 /SimplExpr.bind /=.
-  case he1: (transBeePL_expr_expr e1 fctx bctx g)=> [err1 | ce1 g1 i1] //=.
-  case he2: (transBeePL_expr_expr e2 ce1.1.2 ce1.2 g1)=> [err2 | ce2 g2 i2] //=.
-  move=> [] h1 h2 h3 h4; subst. exists ce1.1.1, ce1.1.2, ce1.2, g1, i1, ce2.1.1, g', i2.
+  case he1: (transBeePL_expr_expr e1 venv fctx bctx g)=> [err1 | ce1 g1 i1] //=.
+  case hf: (fresh_ident (List.map unzip_ident ce1.1.2) max_fresh g1)=> [errf | [cx tag] g2 i2] //=.
+  case he2: (transBeePL_expr_expr e2 (extend venv x cx) ((cx, t, tag) :: ce1.1.2) ce1.2 g2)=> [err2 | ce2 g3 i3] //=.
+  move=> [] h1 h2 h3 h4; subst. exists ce1.1.1, ce1.1.2, ce1.2, g1, i1, ce2.1.1, cx, tag, g2, i2, g', i3.
   split=> //=. + by case: (ce1) => [[a b] c].
   split=> //=. by case: (ce2) he2=> [[a b] c].
 (* cond *)
 + move=> e1 hte1 e2 hte2 e3 hte3 t hte. inversion hte; subst.
   move: H0. rewrite /SimplExpr.bind2 /SimplExpr.bind.
-  case he1: (transBeePL_expr_expr e1 fctx bctx g) => [err1 | ce1 g1 i1] //=.
-  case he2: (transBeePL_expr_expr e2 ce1.1.2 ce1.2 g1) => [err2 | ce2 g2 i2] //=.
-  case he3: (transBeePL_expr_expr e3 ce2.1.2 ce2.2 g2) => [err3 | ce3 g3 i3] //=.
+  case he1: (transBeePL_expr_expr e1 venv fctx bctx g) => [err1 | ce1 g1 i1] //=.
+  case he2: (transBeePL_expr_expr e2 venv ce1.1.2 ce1.2 g1) => [err2 | ce2 g2 i2] //=.
+  case he3: (transBeePL_expr_expr e3 venv ce2.1.2 ce2.2 g2) => [err3 | ce3 g3 i3] //=.
   move=> [] h1 h2 h3 h4; subst. exists ce1.1.1, ce1.1.2, ce1.2, g1, i1, ce2.1.1, ce2.1.2, ce2.2.
   exists g2, i2, ce3.1.1, g', i3. split=> //=.
   + by case: (ce1)=> [[a b] c].
   split=> //=.
   + by case: (ce2) he2=> [[a b] c].
-  split=> //=. by case: (ce3) he3=> [[a b] c].*)
+  split=> //=. by case: (ce3) he3=> [[a b] c].
 Admitted.
 
 Definition is_lvalue (e : Csyntax.expr) : bool :=
@@ -802,57 +807,57 @@ Lemma compilation_preserve_type : forall e venv fctx bctx ce fctx' bctx' g g' i'
 transBeePL_expr_expr e venv fctx bctx g = Res (ce, fctx', bctx') g' i' ->
 transBeePL_type (typeof_expr e) = Csyntax.typeof ce.
 Proof.
-(*move=> e. elim: e=> //=.
+move=> e. elim: e=> //=.
 (* Val *)
-+ move=> v t fctx bctx ce fctx' bctx' g g' i'.
++ move=> v t venv fctx bctx ce fctx' bctx' g g' i'.
   move=> [] h1 h2 h3 h4 /=; subst. by rewrite /Csyntax.typeof.
 (* Var *)
-+ by move=> v t fctx bctx ce fctx' bctx' g g' i' [] h1 h2 h3 h4; subst.
++ by move=> v t venv fctx bctx ce fctx' bctx' g g' i' [] h1 h2 h3 h4; subst.
 (* Const *)
 + move=> [].
   (* bool *)
-  + move=> b t fctx bctx ce fctx' bctx' g g' i' [] h1 h2; subst.  
+  + move=> b t venv fctx bctx ce fctx' bctx' g g' i' [] h1 h2; subst.  
     move: h1. case: ifP=> //=.
     + by move=> hb [] h; subst.
     by move=> hb [] h; subst.
   (* int *)
-  + by move=> i t fctx bctx ce fctx' bctx' g g' i' [] h1 h2 h3 h4; subst.
+  + by move=> i t venv fctx bctx ce fctx' bctx' g g' i' [] h1 h2 h3 h4; subst.
   (* long *)
-  + by move=> i t fctx bctx ce fctx' bctx' g g' i' [] h1 h2 h3 h4; subst.
-  by move=> t fctx bctx ce fctx' bctx' g g' i' [] h1 h2 h3 h4; subst.
+  + by move=> i t venv fctx bctx ce fctx' bctx' g g' i' [] h1 h2 h3 h4; subst.
+  by move=> t venv fctx bctx ce fctx' bctx' g g' i' [] h1 h2 h3 h4; subst.
 (* Call *)
-+ move=> e hin es t fctx bctx ce fctx' bctx' g g' i'.
++ move=> e hin es t venv fctx bctx ce fctx' bctx' g g' i'.
   rewrite /SimplExpr.bind2 /SimplExpr.bind.
-  case he: (transBeePL_expr_expr e fctx bctx g) => [err | [[ce' fe] be] g1 i1] //=.
-  case hes: (transBeePL_expr_exprs transBeePL_expr_expr es fe be) => [err' | [[ces' fes] bes] g2 i2] //=.
+  case he: (transBeePL_expr_expr e venv fctx bctx g) => [err | [[ce' fe] be] g1 i1] //=.
+  case hes: (transBeePL_expr_exprs transBeePL_expr_expr es venv fe be) => [err' | [[ces' fes] bes] g2 i2] //=.
   by move=> [] h1 h2 h3 h4; subst. 
 (* builtin *)
 + move=> [].
   (* ref *)
-  + move=> es t fctx bctx ce fctx' bctx' g g' i'.
+  + move=> es t venv fctx bctx ce fctx' bctx' g g' i'.
     rewrite /SimplExpr.bind2 /SimplExpr.bind.
-    case hes: (transBeePL_expr_exprs transBeePL_expr_expr es fctx bctx g)=> [err' | [[ces' fes] bes] g2 i2] //=.
+    case hes: (transBeePL_expr_exprs transBeePL_expr_expr es venv fctx bctx g)=> [err' | [[ces' fes] bes] g2 i2] //=.
     case hf: (fresh_ident (List.map unzip_ident fes) max_fresh g2)=> [ferr | fi gi ii] //=.
     case: es hes=> [ | e es'] //=. case: es'=> //=. rewrite /SimplExpr.bind2 /SimplExpr.bind.
-    case he: (transBeePL_expr_expr e fctx bctx g) => [err | [[ce' fe] be] g1 i1] //=.
+    case he: (transBeePL_expr_expr e venv fctx bctx g) => [err | [[ce' fe] be] g1 i1] //=.
     move=> [] h1 h2 h3 h4; subst. case h: (ref_to_prim t gi)=> [err | tr gr ir] //=.
     by move=> [] h1 h2 h3 h4 /=; subst. 
   (* deref *)
-  + move=> es t fctx bctx ce fctx' bctx' g g' i'.
+  + move=> es t venv fctx bctx ce fctx' bctx' g g' i'.
     rewrite /SimplExpr.bind2 /SimplExpr.bind /=.
-    case hes: (transBeePL_expr_exprs transBeePL_expr_expr es fctx bctx g)=> [errs | [[ces' fes] bes] g2 i2] //=.
+    case hes: (transBeePL_expr_exprs transBeePL_expr_expr es venv fctx bctx g)=> [errs | [[ces' fes] bes] g2 i2] //=.
     by move=> [] h1 h2 h3 h4; subst.
   (* massgn *)
-  + move=> es t fctx bctx ce fctx' bctx' g g' i'. rewrite /SimplExpr.bind2 /SimplExpr.bind.
-    case hes: (transBeePL_expr_exprs transBeePL_expr_expr es fctx bctx g)=> [errs | [[ces' fes] bes] g2 i2] //=.
+  + move=> es t venv fctx bctx ce fctx' bctx' g g' i'. rewrite /SimplExpr.bind2 /SimplExpr.bind.
+    case hes: (transBeePL_expr_exprs transBeePL_expr_expr es venv fctx bctx g)=> [errs | [[ces' fes] bes] g2 i2] //=.
     by move=> [] h1 h2 h3 h4 /=; subst.
   (* uop *)
-  + move=> u es t fctx bctx ce fctx' bctx' g g' i'. rewrite /SimplExpr.bind2 /SimplExpr.bind.
-    case hes: (transBeePL_expr_exprs transBeePL_expr_expr es fctx bctx g)=> [errs | [[ces' fes] bes] g2 i2] //=.
+  + move=> u es t venv fctx bctx ce fctx' bctx' g g' i'. rewrite /SimplExpr.bind2 /SimplExpr.bind.
+    case hes: (transBeePL_expr_exprs transBeePL_expr_expr es venv fctx bctx g)=> [errs | [[ces' fes] bes] g2 i2] //=.
     by move=> [] h1 h2 h3 h4; subst.
   (* bop *)
-  + move=> u es t fctx bctx ce fctx' bctx' g g' i'. rewrite /SimplExpr.bind2 /SimplExpr.bind.
-    case hes: (transBeePL_expr_exprs transBeePL_expr_expr es fctx bctx g)=> [errs | [[ces' fes] bes] g1 i1] //=.
+  + move=> u es t venv fctx bctx ce fctx' bctx' g g' i'. rewrite /SimplExpr.bind2 /SimplExpr.bind.
+    case hes: (transBeePL_expr_exprs transBeePL_expr_expr es venv fctx bctx g)=> [errs | [[ces' fes] bes] g1 i1] //=.
     case hu: u=> //=. 
     + by move=> [] h1 h2 h3 h4 /=; subst. 
     + by move=> [] h1 h2 h3 h4 /=; subst.
@@ -899,43 +904,43 @@ Proof.
     + by move=> [] h1 h2 h3 h4 /=; subst.
     by move=> [] h1 h2 h3 h4 /=; subst.
   (* Cast *)
-  move=> t es t' fctx bctx ce fctx' bctx' g g' i'. rewrite /SimplExpr.bind2 /SimplExpr.bind /=.
-  case hes: (transBeePL_expr_exprs transBeePL_expr_expr es fctx bctx g)=> [errs | [[ces' fes] bes] g3 i3] //=. by move=> [] h1 h2 h3 h4 /=; subst.
+  move=> t es t' venv fctx bctx ce fctx' bctx' g g' i'. rewrite /SimplExpr.bind2 /SimplExpr.bind /=.
+  case hes: (transBeePL_expr_exprs transBeePL_expr_expr es venv fctx bctx g)=> [errs | [[ces' fes] bes] g3 i3] //=. by move=> [] h1 h2 h3 h4 /=; subst.
 (* Bind *)
-+ move=> x t e hin e' hin' t' fctx bctx ce fctx' bctx' g g' i'. 
-  rewrite /SimplExpr.bind2 /SimplExpr.bind. case: ifP=> //=. 
++ move=> x t e hin e' hin' t' venv fctx bctx ce fctx' bctx' g g' i'. 
+  rewrite /SimplExpr.bind2 /SimplExpr.bind. 
+  case he : (transBeePL_expr_expr e venv fctx bctx g)=> [err | ce1 g1 i1] //=. case: ifP=> //=. 
   + move=> hx.
-    case he : (transBeePL_expr_expr e fctx bctx g)=> [err | ce1 g1 i1] //=. 
-    case he': (transBeePL_expr_expr e' ce1.1.2 ce1.2 g1) => [err1 | ce2 g2 i2] //=.
+    case he': (transBeePL_expr_expr e' venv ce1.1.2 ce1.2 g1) => [err1 | ce2 g2 i2] //=.
     by move=> [] h1 h2 h3 h4 /=; subst.
-  move=> hx.
-  case he : (transBeePL_expr_expr e fctx bctx g)=> [err | ce1 g1 i1] //=. 
-  case he': (transBeePL_expr_expr e' ce1.1.2 ce1.2 g1) => [err1 | ce2 g2 i2] //=.
+  move=> /= hx.
+  case hf: (fresh_ident (List.map unzip_ident ce1.1.2) max_fresh g1) => [errf | [cx tag] g2 i2] //=. 
+  case he': (transBeePL_expr_expr e' (extend venv x cx) ((cx, t, tag) :: ce1.1.2) ce1.2 g2) => [err1 | ce2 g3 i3] //=.
   by move=> [] h1 h2 h3 h4 /=; subst.
 (* Cond *)
-+ move=> e1 hin1 e2 hin2 e3 hin3 t fctx bctx ce fctx' bctx' g g' i'.
++ move=> e1 hin1 e2 hin2 e3 hin3 t venv fctx bctx ce fctx' bctx' g g' i'.
   rewrite /SimplExpr.bind2 /SimplExpr.bind.
-  case he1: (transBeePL_expr_expr e1 fctx bctx g)=> [err1 | ce1 g1 i1] //=.
-  case he2: (transBeePL_expr_expr e2 ce1.1.2 ce1.2 g1) => [err2 | ce2 g2 i2] //=.
-  case he3: (transBeePL_expr_expr e3 ce2.1.2 ce2.2 g2) => [err3 | ce3 g3 i3] //=.
+  case he1: (transBeePL_expr_expr e1 venv fctx bctx g)=> [err1 | ce1 g1 i1] //=.
+  case he2: (transBeePL_expr_expr e2 venv ce1.1.2 ce1.2 g1) => [err2 | ce2 g2 i2] //=.
+  case he3: (transBeePL_expr_expr e3 venv ce2.1.2 ce2.2 g2) => [err3 | ce3 g3 i3] //=.
   by move=> [] h1 h2 h3 h4; subst.
 (* Unit *)
-+ move=> t fctx bctx ce fctx' bctx' g g' i'. by move=> [] h1 h2 h3 h4; subst.
++ move=> t venv fctx bctx ce fctx' bctx' g g' i'. by move=> [] h1 h2 h3 h4; subst.
 (* Addr *)
-+ move=> l i t fctx bctx ce fctx' bctx' g g' i'. by move=> [] h1 h2 h3 h4; subst.
++ move=> l i t venv fctx bctx ce fctx' bctx' g g' i'. by move=> [] h1 h2 h3 h4; subst.
 (* Eapp *)
-+ move=> e ts es t fctx bctx ce fctx' bctx' g g' i'. rewrite /SimplExpr.bind2 /SimplExpr.bind.
-  case he: (transBeePL_expr_exprs transBeePL_expr_expr es fctx bctx g)=> [err | ce1 g1 i1] //=.
++ move=> e ts es t venv fctx bctx ce fctx' bctx' g g' i'. rewrite /SimplExpr.bind2 /SimplExpr.bind.
+  case he: (transBeePL_expr_exprs transBeePL_expr_expr es venv fctx bctx g)=> [err | ce1 g1 i1] //=.
   by move=> [] h1 h2 h3 h4; subst.
 (* Sinit *)
 + admit.
 (* Sfield *)
-+ move=> e hin i t fctx bctx ce fctx' bctx' g g' i'.
++ move=> e hin i t venv fctx bctx ce fctx' bctx' g g' i'.
   rewrite /SimplExpr.bind2 /SimplExpr.bind /=.
-  case he: (transBeePL_expr_expr e fctx bctx g)=> [err1 | ce1 g1 i1] //=.
+  case he: (transBeePL_expr_expr e venv fctx bctx g)=> [err1 | ce1 g1 i1] //=.
   by move=> [] h1 h2 h3 h4; subst.
 (* None *)
-+ move=> t fctx bctx ce fctx' bctx' g g' i'. case: t=> //= p.
++ move=> t venv fctx bctx ce fctx' bctx' g g' i'. case: t=> //= p.
   case: ifP=> //= hot. move=> [] h1 h2 h3 h4 /=; subst.
   by rewrite /Csyntax.typeof /=. 
 (* Some *)
@@ -959,11 +964,11 @@ Proof.
   case he'': (transBeePL_expr_expr e'' ce2.1.2 ce2.2 g3)=> [err2 | ce3 g4 i4] //=.
   by move=> [] h1 h2 h3 h4; subst.*) admit.
 (* Bytes *)
-+ move=> es t fctx bctx ce fctx' bctx' g g' i'. rewrite /SimplExpr.bind2 /SimplExpr.bind.
-  by case he: (transBeePL_expr_exprs transBeePL_expr_expr es fctx bctx g)=> [err | ce' g1 i1] //=.
-move=> h t n t' fctx bctx ce fctx' bctx' g g' i'. rewrite /SimplExpr.bind /=.
++ move=> es t venv fctx bctx ce fctx' bctx' g g' i'. rewrite /SimplExpr.bind2 /SimplExpr.bind.
+  by case he: (transBeePL_expr_exprs transBeePL_expr_expr es venv fctx bctx g)=> [err | ce' g1 i1] //=.
+move=> h t n t' venv fctx bctx ce fctx' bctx' g g' i'. rewrite /SimplExpr.bind /=.
 case ha: (get_array_len t g)=> [err | an g1 i1] //=. case: ifP=> //= hn.
-by move=> [] h1 h2 h3 h4; subst.*)
+by move=> [] h1 h2 h3 h4; subst.
 Admitted.
 
 Lemma convert_rval_type_eq : forall e,
@@ -1057,19 +1062,65 @@ move=> h [] //=.
 by move=> [] //=.
 Qed.
 
+Scheme expr_ind := Induction for BeePL.expr Sort Prop.
+
+Lemma transBeePL_expr_total : (forall se venv fctx1 bctx1 g1,
+ exists (ce' : Csyntax.expr) (fctx'' : seq (ident * type * string)) (bctx'' : bcompiler_ctx) (g'' : generator) (i'' : Ple (gen_next g1) (gen_next g'')),
+    transBeePL_expr_expr se venv fctx1 bctx1 g1 = Res (ce', fctx'', bctx'') g'' i'') /\
+(forall es venv fctx bctx g,
+ exists ces f b g' i', transBeePL_expr_exprs transBeePL_expr_expr es venv fctx bctx g = Res (ces, f, b) g' i').
+Proof.
+Admitted.
+
+Lemma subst_progress_rel : 
+(forall venv x se e e' fctx bctx g ce fctx' bctx' g' i' fctx1 bctx1 g1,
+SubstE x se e e' ->
+transBeePL_expr_expr e venv fctx bctx g = Res (ce, fctx', bctx') g' i' ->
+exists ce' fctx'' bctx'' g'' i'',
+transBeePL_expr_expr e' venv fctx1 bctx1 g1 = Res (ce', fctx'', bctx'') g'' i'') /\
+(forall venv x se es es' fctx bctx g ce fctx' bctx' g' i' fctx1 bctx1 g1,
+SubstEs x se es es' ->
+transBeePL_expr_exprs transBeePL_expr_expr es venv fctx bctx g = Res (ce, fctx', bctx') g' i' ->
+exists ces' fctx'' bctx'' g'' i'',
+transBeePL_expr_exprs transBeePL_expr_expr es' venv fctx1 bctx1 g1 = Res (ces', fctx'', bctx'') g'' i'').
+Proof.
+suff : forall x se, 
+(forall e e', SubstE x se e e' ->
+ forall venv fctx bctx g ce fctx' bctx' g' i' fctx1 bctx1 g1,
+transBeePL_expr_expr e venv fctx bctx g = Res (ce, fctx', bctx') g' i' ->
+exists ce' fctx'' bctx'' g'' i'',
+transBeePL_expr_expr e' venv fctx1 bctx1 g1 = Res (ce', fctx'', bctx'') g'' i'') /\
+(forall es es', SubstEs x se es es' -> 
+ forall venv fctx bctx g ce fctx' bctx' g' i' fctx1 bctx1 g1,
+transBeePL_expr_exprs transBeePL_expr_expr es venv fctx bctx g = Res (ce, fctx', bctx') g' i' ->
+exists ces' fctx'' bctx'' g'' i'',
+transBeePL_expr_exprs transBeePL_expr_expr es' venv fctx1 bctx1 g1 = Res (ces', fctx'', bctx'') g'' i'').
++ admit.
+move=> x se. apply Subst_mutind=> //=.
+(* val *)
++ move=> v t venv fctx bctx g ce fctx' bctx' g' i' fctx1 bctx1 g1 [] h1 h2 h3 h4; subst.
+  have ii: Ple (gen_next g1) (gen_next g1). + by apply Ple_refl.
+  by exists (Eval (trans_bvalue_cvalue v) (transBeePL_type t)), fctx1, bctx1, g1, (Ple_refl (gen_next g1)). 
+(* var (x = y) *)
++ move=> t venv fctx bctx g ce fctx' bctx' g' i' fctx1 bctx1 g1 [] h1 h2 h3 h4; subst.
+  elim: se=> //=.
+  + move=> v vt.
+Admitted.
+
+
 (***** Comparing BeePL big-step semantics with Csyntax big-step semantics *****)
 Lemma bsem_csem_expr_equiv : forall bge cp,
 (forall bp bvm m es m' bvm' bv cge venv fctx bctx ce cvm fctx' bctx' g g' i',
 bsem_exprs bge bp bvm m es m' bvm' bv ->
 BeePL_compcert bp = OK cp ->
 transBeePL_expr_exprs transBeePL_expr_expr es venv fctx bctx g = Res (ce, fctx', bctx') g' i' ->
-match_env bvm cvm ->
+match_env venv bvm cvm ->
 exists tr, eval_exprlist cge cvm m (convert_to_rvals ce) tr m' (get_exprlist bv (map typeof_expr es))) /\
 (forall bp bvm m e m' bvm' bv cge venv fctx bctx ce cvm fctx' bctx' g g' i',
 bsem_expr bge bp bvm m e m' bvm' bv ->
 BeePL_compcert bp = OK cp ->
 transBeePL_expr_expr e venv fctx bctx g = Res (ce, fctx', bctx') g' i' ->
-match_env bvm cvm ->
+match_env venv bvm cvm ->
 exists tr, eval_expression cge cvm m (convert_to_rval ce) tr m' (trans_bvalue_cvalue bv)).
 Proof.
 move=> bge.
@@ -1078,14 +1129,14 @@ suff: (forall bp bvm m es m' bvm' bv,
        forall cp cge fctx bctx ce cvm venv fctx' bctx' g g' i',
          BeePL_compcert bp = OK cp ->
          transBeePL_expr_exprs transBeePL_expr_expr es venv fctx bctx g = Res (ce, fctx', bctx') g' i' ->
-         match_env bvm cvm ->
+         match_env venv bvm cvm ->
          exists tr, eval_exprlist cge cvm m (convert_to_rvals ce) tr m' (get_exprlist bv (map typeof_expr es))) /\
       (forall bp bvm m e m' bvm' bv ,
         bsem_expr bge bp bvm m e m' bvm' bv ->
         forall cp cge fctx bctx ce cvm venv fctx' bctx' g g' i',
           BeePL_compcert bp = OK cp ->
           transBeePL_expr_expr e venv fctx bctx g = Res (ce, fctx', bctx') g' i' ->
-          match_env bvm cvm ->
+          match_env venv bvm cvm ->
           exists tr, eval_expression cge cvm m (convert_to_rval ce) tr m' (trans_bvalue_cvalue bv)).
 + move=> [] hwt1 hwt2. split=> //=.
   + admit.
@@ -1110,10 +1161,10 @@ apply bsem_exprs_bsem_expr_ind_mut=> //=.
     case hc: (chunk_for_volatile_type (transBeePL_type t) Full)=> [c | ] //=.
     + move=> [] tr [] h1 h2. 
       exists (Events.E0 ++ tr). apply eval_expression_intro with (Eval (trans_bvalue_cvalue v) (transBeePL_type t)).
-      + apply eval_valof_volatile with (Csyntax.Evar x (transBeePL_type t)) l Ptrofs.zero Full.
+      + apply eval_valof_volatile with (Csyntax.Evar (resolve venv x) (transBeePL_type t)) l Ptrofs.zero Full.
         + by apply hvt.
         + by apply eval_var.
-        + apply esl_var_local. by have := equiv_local_benv_cenv vm' cvm x l t (transBeePL_type t) hm erefl hvm.
+        + apply esl_var_local. by have := equiv_local_benv_cenv venv vm' cvm x l t (transBeePL_type t) hm erefl hvm.
         + apply deref_loc_volatile with c.
           + by have := access_mode_of_volatile_chunk (transBeePL_type t) c hc.
           + by apply hvt.
@@ -1123,12 +1174,12 @@ apply bsem_exprs_bsem_expr_ind_mut=> //=.
   move=> hl. have hvt' := deref_loc_no_trace_nonvolatile cge (transBeePL_type t) m'' l Ptrofs.zero Full (trans_bvalue_cvalue v) hl.
   by rewrite hvt' in hvt.
   (* type is non volatile *)
-  exists Events.E0. rewrite /convert_to_rval /=. apply eval_expression_intro with (Evalof (Csyntax.Evar x (transBeePL_type t)) (transBeePL_type t)).
+  exists Events.E0. rewrite /convert_to_rval /=. apply eval_expression_intro with (Evalof (Csyntax.Evar (resolve venv x) (transBeePL_type t)) (transBeePL_type t)).
   apply eval_valof.
   + by apply hvt. 
   + by apply eval_var.
   apply esr_rvalof with l Ptrofs.zero Full.
-  + apply esl_var_local. by have := equiv_local_benv_cenv vm' cvm x l t (transBeePL_type t) hm erefl hvm.
+  + apply esl_var_local. by have := equiv_local_benv_cenv venv vm' cvm x l t (transBeePL_type t) hm erefl hvm.
   + by rewrite /Csyntax.typeof.
   + by apply hvt.
   have := deref_addr_translated bge cge t m'' l Ptrofs.zero Full v (transBeePL_type t) (trans_bvalue_cvalue v) hd erefl erefl.
@@ -1144,11 +1195,11 @@ apply bsem_exprs_bsem_expr_ind_mut=> //=.
     case hc: (chunk_for_volatile_type (transBeePL_type t) Full)=> [c | ] //=.
     + move=> [] tr [] h1 h2. 
       exists (Events.E0 ++ tr). apply eval_expression_intro with (Eval (trans_bvalue_cvalue v) (transBeePL_type t)).
-      + apply eval_valof_volatile with (Csyntax.Evar x (transBeePL_type t)) l Ptrofs.zero Full.
+      + apply eval_valof_volatile with (Csyntax.Evar (resolve venv x) (transBeePL_type t)) l Ptrofs.zero Full.
         + by apply hvt.
         + by apply eval_var.
-        + apply esl_var_global. by have := equiv_global_benv_cenv vm' cvm x hm hvm.
-        + have hg' := symbols_preserved bge cge x. by rewrite hg in hg'.
+        + apply esl_var_global. by have := equiv_global_benv_cenv venv vm' cvm x hm hvm.
+        + have hg' := symbols_preserved venv bge cge x. by rewrite hg in hg'.
         + apply deref_loc_volatile with c.
           + by have := access_mode_of_volatile_chunk (transBeePL_type t) c hc.
           + by apply hvt.
@@ -1158,13 +1209,13 @@ apply bsem_exprs_bsem_expr_ind_mut=> //=.
   move=> hl. have hvt' := deref_loc_no_trace_nonvolatile cge (transBeePL_type t) m'' l Ptrofs.zero Full (trans_bvalue_cvalue v) hl.
   by rewrite hvt' in hvt.
   (* type is non volatile *)
-  exists Events.E0. rewrite /convert_to_rval /=. apply eval_expression_intro with (Evalof (Csyntax.Evar x (transBeePL_type t)) (transBeePL_type t)).
+  exists Events.E0. rewrite /convert_to_rval /=. apply eval_expression_intro with (Evalof (Csyntax.Evar (resolve venv x) (transBeePL_type t)) (transBeePL_type t)).
   apply eval_valof.
   + by apply hvt. 
   + by apply eval_var.
   apply esr_rvalof with l Ptrofs.zero Full.
-  + apply esl_var_global. by have := equiv_global_benv_cenv vm' cvm x hm hvm.
-  + have hg' := symbols_preserved bge cge x. by rewrite hg in hg'.
+  + apply esl_var_global. by have := equiv_global_benv_cenv venv vm' cvm x hm hvm.
+  + have hg' := symbols_preserved venv bge cge x. by rewrite hg in hg'.
   + by simpl. 
   + by apply hvt.
   have := deref_addr_translated bge cge t m'' l Ptrofs.zero Full v (transBeePL_type t) (trans_bvalue_cvalue v) hd erefl erefl.
@@ -1327,16 +1378,16 @@ apply bsem_exprs_bsem_expr_ind_mut=> //=.
 (* bind *)
 + move=> p vm m x e1 m' m'' v e2 e2' v' tx he1 hin1 hx hst he2 hin2 cp cge fctx bctx ce cvm venv fctx' bctx' g g' i' hp hte hm.
   have [htr1 htr2] := trans_expr_expr_ind.
-  move: (htr1 (Bind x tx e1 e2 (typeof_expr e2)) venv fctx bctx ce fctx' bctx' g g' i' hte)=> [] ce1 [] fctx1 [] bctx1 [] g1 [] i1 [] ce2 [] g2 [] i2 [] hce1 [] hce2.
-  move: (hin1 cp cge fctx bctx ce1 cvm venv fctx1 bctx1 g g1 i1 hp hce1 hm)=> [] tr1 hce3; subst.
-  case: ifP=> //= hxeq.
+  move: (htr1 (Bind x tx e1 e2 (typeof_expr e2)) venv fctx bctx ce fctx' bctx' g g' i' hte). case: ifP=> //= hxeq.
   (* !x = _ *)
-  + admit.
-  (* x = _ *) (* bind as seq done *)
+  + move=> [] ce1 [] fctx1 [] bctx1 [] g1 [] i1 [] ce2 [] cx [] tag [] g2 [] i2 [] g3 [] i3 [] hce1 [] hf [] hce2 heq /=; subst.
+    rewrite /=. move: (hin1 cp cge fctx bctx ce1 cvm venv fctx1 bctx1 g g1 i1 hp hce1 hm)=> [] tr1 hc1.
+    move: (hin2 cp cge  ((cx, tx, tag) :: fctx1) bctx1 ce2 cvm venv fctx' bctx' g2 g3 i3 hp). admit.
+  (* x = _ *) (* bind as seq *) (* done *)
   move=> p vm m x e1 m' m'' v e2 v' tx he1 hin1 hx he2 hin2 cp cge fctx bctx ce cvm venv fctx' bctx' g g' i' hp hte hm.
   have [htr1 htr2] := trans_expr_expr_ind.
-  move: (htr1 (Bind x tx e1 e2 (typeof_expr e2)) venv fctx bctx ce fctx' bctx' g g' i' hte)=> [] ce1 [] fctx1 [] bctx1 [] g1 [] i1 [] ce2 [] g2 [] i2 [] hce1 [] hce2.
-  rewrite /ident_of_string /= hx /=. move=> heq; subst.
+  move: (htr1 (Bind x tx e1 e2 (typeof_expr e2)) venv fctx bctx ce fctx' bctx' g g' i' hte). 
+  rewrite /ident_of_string /= hx /=. move=> heq; subst. move: heq. move=> [] ce1 [] fctx1 [] bctx1 [] g1 [] i1 [] ce2 [] g2 [] i2 [] hce1 [] hce2.
   move: (hin1 cp cge fctx bctx ce1 cvm venv fctx1 bctx1 g g1 i1 hp hce1 hm)=> [] tr1 hce3; subst.
   move: (hin2 cp cge fctx1 bctx1 ce2 cvm venv fctx' bctx' g1 g2 i2 hp hce2 hm)=> [] tr2 hce4; subst.
   exists (tr1 ++ tr2). rewrite /=. inversion hce3; subst. inversion hce4; subst.
@@ -1346,11 +1397,11 @@ apply bsem_exprs_bsem_expr_ind_mut=> //=.
   have -> := convert_rval_type_eq ce2. by rewrite ht.
   by apply H2.
 (* cond *) (* done *)
-+ move=> p vm m e1 e2 e3 t m' vb ct1 v' v v'' m'' he1 hin1 ht1 hb he2 hin2 hs hv cp cge fctx bctx ce
++ (*move=> p vm m e1 e2 e3 t m' vb ct1 v' v v'' m'' he1 hin1 ht1 hb he2 hin2 hs hv cp cge fctx bctx ce
          cvm venv fctx' bctx' g g' i' hp he hm.
   have [htr1 htr2] := trans_expr_expr_ind.
   move: (htr1 (Cond e1 e2 e3 t) venv fctx bctx ce fctx' bctx' g g' i' he)=> [] ce1 [] fctx1 [] bctx1 [] g1 [] i1 [] ce2 [] fctx2 [] bctx2 [] g2 [] i2
-  [] ce3 [] g3 [] i3 [] hte1 [] hte2 [] hte [] /andP [] hteq1 hteq2 heq; subst.
+  [] ce3 [] g3 [] i3 [] hte1 [] hte2 [] hte. [] /andP [] hteq1 hteq2 heq; subst.
   move: (hin1 cp cge fctx bctx ce1 cvm venv fctx1 bctx1 g g1 i1 hp hte1 hm)=> [] tr1 hve1.
   move: (hin2 cp cge fctx1 bctx1 ce2 cvm venv fctx2 bctx2 g1 g2 i2 hp hte2 hm) => [] tr2 hve2.
   (* true *)
@@ -1379,7 +1430,7 @@ apply bsem_exprs_bsem_expr_ind_mut=> //=.
       have hteq3 := convert_rval_type_eq ce3. rewrite hteq3 /=.
       have <- := eq_type_trans t (typeof_expr e3) (Csyntax.typeof ce3) hteq2 hteq''. rewrite -hteq''. 
     by apply hs. 
-  have -> := bv_cv_reflex v'' v hv. by apply esr_val. 
+  have -> := bv_cv_reflex v'' v hv. by apply esr_val.*) 
 Admitted.
 
 (***** Comparing BeePL big-step semantics with Csyntax big-step semantics *****)
@@ -1387,7 +1438,7 @@ Lemma bsem_csem_stmt_equiv :
 forall venv bge cge p bcmp fctx bctx bvm m e m' bvm' bv ce tr cvm fctx' bctx' o g g' i',
 bsem_expr bge p bvm m e m' bvm' bv ->
 transBeePL_expr_st bcmp e venv fctx bctx g = Res (ce, fctx', bctx') g' i'  ->
-match_env bvm cvm ->
+match_env venv bvm cvm ->
 exec_stmt cge cvm m ce tr m' o.
 Proof.
 Admitted.
